ulib/experimental/FStar.MSTTotal.fst
@@ -18,27 +18,10 @@ module FStar.MSTTotal
 
 module P = FStar.Preorder
 
+open FStar.Monotonic.Pure
+
 type pre_t (state:Type u#2) = state -> Type0
 type post_t (state:Type u#2) (a:Type u#a) = state -> a -> state -> Type0
-
-unfold
-let req_ens_to_wp0 (#a:Type) (#state:Type u#2)
-  (rel:P.preorder state) (req:pre_t state) (ens:post_t state a) (s0:state)
-  (p:pure_post (a & state))
-  = req s0 /\
-    (forall (x:a) (s1:state). (ens s0 x s1 /\ rel s0 s1) ==> p (x, s1))
-
-let req_ens_to_wp0_monotonic (#a:Type) (#state:Type u#2)
-  (rel:P.preorder state) (req:pre_t state) (ens:post_t state a) (s0:state)
-  : Lemma (pure_wp_monotonic (req_ens_to_wp0 rel req ens s0))
-  = reveal_opaque (`%pure_wp_monotonic) (pure_wp_monotonic #(a & state))
-
-unfold
-let req_ens_to_wp (#a:Type) (#state:Type u#2)
-  (rel:P.preorder state) (req:pre_t state) (ens:post_t state a) (s0:state)
-  : pure_wp (a & state)
-  = req_ens_to_wp0_monotonic rel req ens s0;
-    req_ens_to_wp0 rel req ens s0
 
 type repr
       (a:Type)
@@ -48,7 +31,10 @@ type repr
       (ens:post_t state a)
     =
   s0:state ->
-  PURE (a & state) (req_ens_to_wp rel req ens s0)
+  PURE (a & state)
+    (coerce_to_pure_wp (fun p ->
+                        req s0 /\
+                        (forall (x:a) (s1:state). (ens s0 x s1 /\ rel s0 s1) ==> p (x, s1))))
 
 let return
       (a:Type)
@@ -191,7 +177,7 @@ let lift_pure_mst_total
       (fun s0 -> wp (fun _ -> True))
       (fun s0 x s1 -> wp (fun _ -> True) /\  (~ (wp (fun r -> r =!= x \/ s0 =!= s1))))
     =
-  FStar.Monotonic.Pure.wp_monotonic_pure ();
+  elim_pure_wp_monotonicity wp;
   fun s0 ->
     let x = f () in
     x, s0
